examples/low-level/crypto/Crypto.AEAD.fst
@@ -23,305 +23,133 @@ open Flag
 open Crypto.Symmetric.PRF
 open Crypto.AEAD.Encoding 
 open Crypto.AEAD.Invariant
-(* open Crypto.AEAD.Lemmas *)
-(* open Crypto.AEAD.Lemmas.Part2 *)
-(* open Crypto.AEAD.Lemmas.Part3 *)
-open Crypto.AEAD.Wrappers
+(* open Crypto.AEAD.Wrappers *)
 
-module HH = FStar.HyperHeap
-module HS = FStar.HyperStack
-
-module MAC = Crypto.Symmetric.MAC
-module CMA = Crypto.Symmetric.UF1CMA
-
-module Plain = Crypto.Plain
+module HH     = FStar.HyperHeap
+module HS     = FStar.HyperStack
+module MAC    = Crypto.Symmetric.MAC
+module CMA    = Crypto.Symmetric.UF1CMA
+module Plain  = Crypto.Plain
 module Cipher = Crypto.Symmetric.Cipher
-module PRF = Crypto.Symmetric.PRF
+module PRF    = Crypto.Symmetric.PRF
+module Enxor  = Crypto.AEAD.Enxor
 
-type region = rgn:HH.rid {HS.is_eternal_region rgn}
-
-let ctr x = PRF.(x.ctr)
-
-// Overview of the stateful invariant:
-//
-// We allocate AEAD logs at the writer (complying with our `local modifier' discipline)
-// We allocate all PRF tables in a global private region (to escape that discipline)
-
-// Global state invariant: 
-// for all ideal instances of AEAD, 
-// - their regions and PRFs tables are pairwise disjoint; and
-// - their PRF table contents correctly refines their AEAD logs,
-//     (up to early decryptor allocations in initial state)
-
-// This invariant depends only on AEAD-writer regions and the PRF region. 
-//
-// During AE encrypt, the invariant is eventually restored as we extend the AEAD log, 
-// using a precise record of all entries added to the PRF table during encryption.
-//
-// During AE decrypt, the only interesting case is when early
-// verification fails: the invariant is restored for an extended PRF
-// state with an extra MAC in its initial state.
-//
-// For convenience, 'refines' relies on both the log and the table being ordered chronologically.
-
-// TODO `Functional' correctness? (actually a witnessed, stable property)
-// c = encryptT h i st nonce ad (real_or_zero i p) 
-//
-// Ideally, this depends on the (increasing) states of 
-// both the PRF and its MACs, and may follow from the global invariant.
-//
-// Really, this depends on the functional correctness of PRF. 
-// Needed: prf_read returning a ghost of the actual underlying block. 
-//let sub s start len = Seq.slice start (start+len) s // more convenient? 
-
-val gen: i:id -> rgn:region -> ST (state i Writer)
-  (requires (fun _ -> True))
-  (ensures  (fun h0 st h1 -> True))
+val gen: 
+  i:id -> 
+  rgn:eternal_region -> 
+  ST (aead_state i Writer)
+     (requires (fun _ -> True))
+     (ensures  (fun h0 st h1 -> True))
 let gen i rgn = 
   let prf = PRF.gen rgn i in 
   if Flag.prf i then recall (PRF.itable i prf);
-  let log = ralloc rgn (Seq.createEmpty #(entry i)) in
+  let log = ralloc rgn (Seq.createEmpty #(aead_entry i)) in
   let ak = if CMA.skeyed i then Some (PRF.prf_sk0 #i prf) else None in 
-  State #i #Writer #rgn log prf ak
+  AEADState #i #Writer #rgn log prf ak
 
-val coerce: i:id{~(prf i)} -> rgn:region -> key:lbuffer (v (PRF.keylen i)) -> ST (state i Writer)
-  (requires (fun h -> Buffer.live h key))
-  (ensures  (fun h0 st h1 -> True))
+val coerce: 
+    i:id{~(prf i)} -> 
+    rgn:eternal_region -> 
+    key:lbuffer (v (PRF.keylen i)) -> 
+    ST (aead_state i Writer)
+       (requires (fun h -> Buffer.live h key))
+       (ensures  (fun h0 st h1 -> True))
 let coerce i rgn key = 
   let prf = PRF.coerce rgn i key in
   if Flag.prf i then recall (PRF.itable i prf);
-  let log = ralloc rgn (Seq.createEmpty #(entry i)) in // Shouldn't exist
+  let log = ralloc rgn (Seq.createEmpty #(aead_entry i)) in // Shouldn't exist ... NS??
   let ak = if CMA.skeyed i then Some (PRF.prf_sk0 #i prf) else None in 
-  State #i #Writer #rgn log prf ak
+  AEADState #i #Writer #rgn log prf ak
 
-#reset-options "--z3rlimit 20"
-
-val genReader: #i:id -> st:state i Writer -> ST (state i Reader)
+val genReader: #i:id -> st:aead_state i Writer -> ST (aead_state i Reader)
   (requires (fun _ -> True))
   (ensures  (fun _ _ _ -> True))
 let genReader #i st =
-  State #i #Reader #st.log_region st.log st.prf st.ak
+  AEADState #i #Reader #st.log_region st.log st.prf st.ak
 
-val leak: #i:id{~(prf i)} -> st:state i Writer -> ST (lbuffer (v (PRF.statelen i)))
+val leak: #i:id{~(prf i)} -> st:aead_state i Writer -> ST (lbuffer (v (PRF.statelen i)))
   (requires (fun _ -> True))
   (ensures  (fun _ _ _ -> True))
 let leak #i st = PRF.leak st.prf
 
-let prf_state (#i:id) (#rw:rw) (e:state i rw) : PRF.state i = State?.prf e
 ////////////////////////////////////////////////////////////////////////////////
+let fresh_nonce (#i:id) (#rw:rw) 
+		(n:Cipher.iv (alg i)) 
+		(st:aead_state i rw)
+		(h:mem) = 
+   let entries = HS.sel h st.log in		  
+   None? (find_aead_entry n entries)
 
 #reset-options "--z3rlimit 400 --initial_fuel 0 --max_fuel 0 --initial_ifuel 0 --max_ifuel 0"
-val extend_refines_aux: (i:id) -> (st:state i Writer) -> (nonce:Cipher.iv (alg i)) ->
-		       (aadlen: UInt32.t {aadlen <=^ aadmax}) ->
-		       (aad: lbuffer (v aadlen)) ->
-                       (len:nat{len<>0}) -> (plain:plainBuffer i len) -> (cipher:lbuffer (len + v MAC.taglen)) ->
-		       (h0:mem) ->
-                       (h1:mem{Buffer.live h1 aad /\ Plain.live h1 plain /\ Buffer.live h1 cipher}) ->
-    Lemma (requires ( safeId i ==> (
-		      let mac_rgn = st.prf.mac_rgn in
-      		      let entries_0 = HS.sel h0 st.log in 
-		      let blocks_0 = HS.sel h0 (PRF.itable i st.prf) in
-		      let table_1 = HS.sel h1 (PRF.itable i st.prf) in
-		      Seq.length table_1 > Seq.length blocks_0 /\ (
-		      let blocks_1 = Seq.slice table_1 (Seq.length blocks_0) (Seq.length table_1) in
-
-     		      let p = Plain.sel_plain h1 (u len) plain in
-		      let c_tagged = Buffer.as_seq h1 cipher in
-	              let c, tag = SeqProperties.split c_tagged len in
-		      let ad = Buffer.as_seq h1 aad in
-  		      let entry = Entry nonce ad len p c_tagged in
-		      pre_refines_one_entry i st nonce len plain cipher h0 h1 /\
-		      inv h0 st /\
-		      refines_one_entry #_ #i h1 entry blocks_1 /\
-      		      HS.modifies_ref mac_rgn TSet.empty h0 h1 /\
-		      HS.live_region h1 mac_rgn))))
-		      
-          (ensures ( safeId i ==> (
-		      let mac_rgn = st.prf.mac_rgn in
-      		      let entries_0 = HS.sel h0 st.log in 
-		      let table_1 = HS.sel h1 (PRF.itable i st.prf) in
-     		      let p = Plain.sel_plain h1 (u len) plain in
-		      let c_tagged = Buffer.as_seq h1 cipher in
-	              let c, tag = SeqProperties.split c_tagged len in
-		      let ad = Buffer.as_seq h1 aad in
-  		      let entry = Entry nonce ad len p c_tagged in
-		      refines h1 i mac_rgn (SeqProperties.snoc entries_0 entry) table_1)))
-let extend_refines_aux i st nonce aadlen aad len plain cipher h0 h1 = 
-  if safeId i then
-     let mac_rgn = st.prf.mac_rgn in
-     let entries_0 = HS.sel h0 st.log in 
-     let blocks_0 = HS.sel h0 (PRF.itable i st.prf) in
-     let table_1 = HS.sel h1 (PRF.itable i st.prf) in
-     let blocks_1 = Seq.slice table_1 (Seq.length blocks_0) (Seq.length table_1) in
-     let p = Plain.sel_plain h1 (u len) plain in
-     let c_tagged = Buffer.as_seq h1 cipher in
-     let c, tag = SeqProperties.split c_tagged len in
-     let ad = Buffer.as_seq h1 aad in
-     let entry = Entry nonce ad len p c_tagged in
-     extend_refines h0 i mac_rgn entries_0 blocks_0 entry blocks_1 h1
-
-#reset-options "--z3rlimit 400 --initial_fuel 0 --max_fuel 0 --initial_ifuel 0 --max_ifuel 0"
+let aadlen = x:UInt32.t{x <=^ aadmax}
 let encrypt_ensures' (regions:Set.set HH.rid)
-		     (i:id) (st:state i Writer)
+		     (#i:id) (st:aead_state i Writer)
 		     (n: Cipher.iv (alg i))
- 		     (aadlen: UInt32.t {aadlen <=^ aadmax})
+		     (#aadlen:aadlen)
 		     (aad: lbuffer (v aadlen))
-		     (plainlen: UInt32.t {plainlen <> 0ul /\ safelen i (v plainlen) (ctr_0 i +^ 1ul)})
+		     (#plainlen: UInt32.t)
 		     (plain: plainBuffer i (v plainlen))
 		     (cipher_tagged:lbuffer (v plainlen + v MAC.taglen))
-		     (h0:mem) (h5:mem) = 
-     Buffer.live h5 aad /\
-     Buffer.live h5 cipher_tagged /\
-     Plain.live h5 plain /\
-     my_inv st h5 /\
-     HS.modifies_transitively regions h0 h5 /\ (
-     safeId i ==>  (
-       let aad = Buffer.as_seq h5 aad in
-       let p = Plain.sel_plain h5 plainlen plain in
-       let c = Buffer.as_seq h5 cipher_tagged in
-       HS.sel h5 st.log == SeqProperties.snoc (HS.sel h0 st.log) (Entry n aad (v plainlen) p c)))
+		     (h0:mem) (h1:mem) = 
+    enc_dec_liveness st aad plain cipher_tagged h1 /\
+    inv st h1 /\
+    HS.modifies_transitively regions h0 h1 /\
+    (safeId i ==>  (
+       let aad = Buffer.as_seq h1 aad in
+       let p = Plain.sel_plain h1 plainlen plain in
+       let c = Buffer.as_seq h1 cipher_tagged in
+       HS.sel h1 st.log == SeqProperties.snoc (HS.sel h0 st.log) (AEADEntry n aad (v plainlen) p c)))
+       
+    
+     (* Buffer.live h5 aad /\ *)
+     (* Buffer.live h5 cipher_tagged /\ *)
+     (* Plain.live h5 plain /\ *)
+     (* my_inv st h5 /\ *)
+     (* HS.modifies_transitively regions h0 h5 /\ ( *)
+     (* safeId i ==>  ( *)
+     (*   let aad = Buffer.as_seq h5 aad in *)
+     (*   let p = Plain.sel_plain h5 plainlen plain in *)
+     (*   let c = Buffer.as_seq h5 cipher_tagged in *)
+     (*   HS.sel h5 st.log == SeqProperties.snoc (HS.sel h0 st.log) (Entry n aad (v plainlen) p c))) *)
 
-let encrypt_ensures_tip (i:id) (st:state i Writer)
+(* let encrypt_ensures_tip (i:id) (st:state i Writer) *)
+(* 		     (n: Cipher.iv (alg i)) *)
+(*  		     (aadlen: UInt32.t {aadlen <=^ aadmax}) *)
+(* 		     (aad: lbuffer (v aadlen)) *)
+(* 		     (plainlen: UInt32.t {plainlen <> 0ul /\ safelen i (v plainlen) (ctr_0 i +^ 1ul)}) *)
+(* 		     (plain: plainBuffer i (v plainlen)) *)
+(* 		     (cipher_tagged:lbuffer (v plainlen + v MAC.taglen)) *)
+(* 		     (h0:mem) (h5:mem) = *)
+(*   encrypt_ensures' (Set.as_set [st.log_region; Buffer.frameOf cipher_tagged; HS.(h5.tip)]) *)
+(*     i st n aadlen aad plainlen plain cipher_tagged h0 h5 *)
+
+let encrypt_ensures  (#i:id) (st:aead_state i Writer)
 		     (n: Cipher.iv (alg i))
- 		     (aadlen: UInt32.t {aadlen <=^ aadmax})
+		     (#aadlen:aadlen)
 		     (aad: lbuffer (v aadlen))
-		     (plainlen: UInt32.t {plainlen <> 0ul /\ safelen i (v plainlen) (ctr_0 i +^ 1ul)})
+		     (#plainlen: UInt32.t)
 		     (plain: plainBuffer i (v plainlen))
 		     (cipher_tagged:lbuffer (v plainlen + v MAC.taglen))
-		     (h0:mem) (h5:mem) =
-  encrypt_ensures' (Set.as_set [st.log_region; Buffer.frameOf cipher_tagged; HS.(h5.tip)])
-    i st n aadlen aad plainlen plain cipher_tagged h0 h5
-
-let encrypt_ensures  (i:id) (st:state i Writer)
-		     (n: Cipher.iv (alg i))
- 		     (aadlen: UInt32.t {aadlen <=^ aadmax})
-		     (aad: lbuffer (v aadlen))
-		     (plainlen: UInt32.t {plainlen <> 0ul /\ safelen i (v plainlen) (ctr_0 i +^ 1ul)})
-		     (plain: plainBuffer i (v plainlen))
-		     (cipher_tagged:lbuffer (v plainlen + v MAC.taglen))
-		     (h0:mem) (h5:mem) =
-  encrypt_ensures' (Set.as_set [st.log_region; Buffer.frameOf cipher_tagged])
-    i st n aadlen aad plainlen plain cipher_tagged h0 h5
-
-val finish_after_mac: h0:mem -> h3:mem -> i:id -> st:state i Writer -> 
-		      n: Cipher.iv (alg i) ->
-		      aadlen: UInt32.t {aadlen <=^ aadmax} -> 
-		      aad: lbuffer (v aadlen) -> 
-		      plainlen: UInt32.t {plainlen <> 0ul /\ safelen i (v plainlen) (ctr_0 i +^ 1ul)} -> 
-		      plain: plainBuffer i (v plainlen) -> 
-		      cipher_tagged:lbuffer (v plainlen + v MAC.taglen) ->
-		      ak:CMA.state (i, n) -> acc:CMA.accBuffer (i, n) -> tag:MAC.tagB -> ST unit
-  (requires (fun h4 -> 
-    let cipher = Buffer.sub cipher_tagged 0ul plainlen in
-    let x0 = {iv=n; ctr=ctr_0 i} in
-    HS.(h0.tip = h4.tip) /\
-    HH.disjoint (HS.(h4.tip)) st.log_region /\
-    HH.disjoint (HS.(h4.tip)) (Buffer.frameOf cipher_tagged) /\
-    HS.modifies_transitively (Set.as_set [st.log_region; Buffer.frameOf cipher_tagged; HS.(h4.tip)]) h0 h3 /\
-    HS.modifies_ref st.prf.mac_rgn TSet.empty h0 h3 /\
-    (prf i ==> none_above ({iv=n; ctr=ctr_0 i}) st.prf h0) /\ // The nonce must be fresh!
-    pre_refines_one_entry i st n (v plainlen) plain cipher_tagged h0 h3 /\
-    mac_ensures (i, n) ak acc tag h3 h4 /\
-    (my_inv st h0) /\
-    (CMA.(ak.region = st.prf.mac_rgn)) /\
-    (safeId i ==> ~ (m_contains (CMA.(ilog ak.log)) h0)) /\
-    (prf i ==> HS.frameOf (PRF.itable i st.prf) <> Buffer.frameOf cipher_tagged) /\
-    (Buffer.disjoint (Plain.as_buffer plain) cipher_tagged) /\
-    (Buffer.disjoint aad cipher_tagged) /\
-    (HH.disjoint (Buffer.frameOf (Plain.as_buffer plain)) st.log_region) /\
-    (HH.disjoint (Buffer.frameOf cipher_tagged) st.log_region) /\  
-    (Buffer.live h3 cipher_tagged) /\
-    (Plain.live h3 plain) /\
-    (Buffer.live h3 aad) /\
-    (tag == Buffer.sub cipher_tagged plainlen MAC.taglen) /\
-    (mac_log ==> 
-      (h3 `HS.contains` CMA.alog acc) /\
-      (HS.frameOf (CMA.alog acc) = HS.(h3.tip)) /\
-      FStar.HyperStack.sel h3 (CMA.alog acc) ==
-      encode_both i aadlen (Buffer.as_seq h3 aad) plainlen (Buffer.as_seq h3 cipher)) /\ //from accumulate
-    (safeId i ==>
-	HS.modifies_ref st.log_region (TSet.singleton (FStar.Heap.Ref (HS.as_ref (PRF.itable i st.prf)))) h0 h3 /\ (
-	let tab = HS.sel h3 (PRF.itable i st.prf) in
-	match PRF.find_mac tab x0 with
-	| None -> False
-	| Some mac_st -> mac_st == ak))))
-   (ensures (fun _ _ h5 -> 
-              encrypt_ensures_tip i st n aadlen aad plainlen plain cipher_tagged h0 h5))
-
-#reset-options "--z3rlimit 1000 --initial_fuel 0 --max_fuel 0 --initial_ifuel 0 --max_ifuel 0"
-let finish_after_mac h0 h3 i st n aadlen aad plainlen plain cipher_tagged ak acc tag = 
-  if prf i then recall (itable i st.prf);
-  if safeId i then recall st.log;
-  let h4 = get () in
-  if safeId i 
-  then begin
-    intro_mac_refines i st n aad plain cipher_tagged h4;
-    modifies_fresh_empty i n st.prf.mac_rgn ak h0 h3 h4;
-    frame_pre_refines i st n (v plainlen) plain cipher_tagged h0 h3 h4;
-    pre_refines_to_refines i st n aadlen aad (v plainlen) plain cipher_tagged h0 h4;
-    extend_refines_aux i st n aadlen aad (v plainlen) plain cipher_tagged h0 h4;
-    refines_to_inv i st n aadlen aad plainlen plain cipher_tagged
-  end
-  else FStar.Classical.move_requires (Buffer.lemma_reveal_modifies_1 tag h3) h4
-
-let encrypt_ensures_push_pop (i:id) (st:state i Writer)
-		    (n: Cipher.iv (alg i))
-		    (aadlen: UInt32.t {aadlen <=^ aadmax})
-		    (aad: lbuffer (v aadlen))
-		    (plainlen: UInt32.t {plainlen <> 0ul /\ safelen i (v plainlen) (ctr_0 i +^ 1ul)})
-		    (plain: plainBuffer i (v plainlen))
-		    (cipher_tagged:lbuffer (v plainlen + v MAC.taglen))
-		    (h:mem) (h0:mem) (h5:mem)
-   : Lemma (requires (let open FStar.HyperStack in
-		      fresh_frame h h0 /\
-		      HH.disjoint st.log_region h0.tip /\
-		      HH.disjoint (Buffer.frameOf (Plain.as_buffer plain)) h0.tip /\
-     		      HH.disjoint (Buffer.frameOf aad) h0.tip /\
-      		      HH.disjoint (Buffer.frameOf cipher_tagged) h0.tip /\
-		      encrypt_ensures_tip i st n aadlen aad plainlen plain cipher_tagged h0 h5))
-	   (ensures (HS.poppable h5 /\
-		     encrypt_ensures i st n aadlen aad plainlen plain cipher_tagged h (HS.pop h5)))
-   = if safeId i
-     then frame_refines i st.prf.mac_rgn (HS.sel h5 st.log) (HS.sel h5 (PRF.itable i st.prf)) h5 (HS.pop h5)
-     
+		     (h0:mem) (h1:mem) = 
+  encrypt_ensures' (Set.as_set [st.log_region; Buffer.frameOf cipher_tagged]) st n aad plain cipher_tagged h0 h1
 
 val encrypt:
-  i: id -> st:state i Writer ->
+  i: id -> st:aead_state i Writer ->
   n: Cipher.iv (alg i) ->
-  aadlen: UInt32.t {aadlen <=^ aadmax} ->
+  aadlen: aadlen ->
   aad: lbuffer (v aadlen) ->
-  plainlen: UInt32.t {plainlen <> 0ul /\ safelen i (v plainlen) (ctr_0 i +^ 1ul)} ->
+  plainlen: UInt32.t {plainlen <> 0ul /\ safelen i (v plainlen) (otp_offset i)} ->
   plain: plainBuffer i (v plainlen) ->
-  cipher_tagged:lbuffer (v plainlen + v MAC.taglen)
-  {
-    Buffer.disjoint aad cipher_tagged /\
-    Buffer.disjoint (Plain.as_buffer plain) aad /\
-    Buffer.disjoint (Plain.as_buffer plain) cipher_tagged /\
-    HH.disjoint (Buffer.frameOf (Plain.as_buffer plain)) st.log_region /\
-    HH.disjoint (Buffer.frameOf cipher_tagged) st.log_region /\
-    HH.disjoint (Buffer.frameOf aad) st.log_region /\
-    HS.is_eternal_region st.log_region /\
-    HS.is_eternal_region (Buffer.frameOf cipher_tagged) /\ // why?
-    HS.is_eternal_region (Buffer.frameOf (Plain.as_buffer plain)) /\ //why?
-    HS.is_eternal_region (Buffer.frameOf aad) /\ //why?
-    st.log_region <> HH.root /\
-    Buffer.frameOf cipher_tagged <> HH.root /\
-    Buffer.frameOf aad <> HH.root /\
-    Buffer.frameOf (Plain.as_buffer plain) <> HH.root
-  }
-  ->
+  cipher_tagged:lbuffer (v plainlen + v MAC.taglen) ->
   ST unit
-  (requires (fun h ->
-    let prf_rgn = st.prf.rgn in
-    my_inv st h /\
-    Buffer.live h aad /\
-    Buffer.live h cipher_tagged /\
-    Plain.live h plain /\
-    st.log_region  `HS.is_in` (HS.(h.h)) /\
-    (prf i ==> none_above ({iv=n; ctr=ctr_0 i}) st.prf h) // The nonce must be fresh!
-   ))
-  (ensures (fun h0 _ h5 ->
-    encrypt_ensures i st n aadlen aad plainlen plain cipher_tagged h0 h5))
+    (requires (fun h ->
+	enc_dec_separation st aad plain cipher_tagged /\
+	enc_dec_liveness st aad plain cipher_tagged h /\
+	fresh_nonce n st h /\
+	inv st h))
+    (ensures (fun h0 _ h1 ->
+	enc_dec_liveness st aad plain cipher_tagged h1 /\
+	encrypt_ensures st n aad plain cipher_tagged h0 h1))
 let encrypt i st n aadlen aad plainlen plain cipher_tagged =
   let h_init = get() in
   push_frame(); 
@@ -1147,3 +975,38 @@ let decrypt i st iv aadlen aad plainlen plain cipher_tagged =
   frame_decrypt_ok iv st aad plain cipher_tagged verified h4;
   chain_modification i iv st aad plain cipher_tagged h_init h0 h1 h2 h3 h4;
   verified
+
+
+
+
+// Overview of the stateful invariant:
+//
+// We allocate AEAD logs at the writer (complying with our `local modifier' discipline)
+// We allocate all PRF tables in a global private region (to escape that discipline)
+
+// Global state invariant: 
+// for all ideal instances of AEAD, 
+// - their regions and PRFs tables are pairwise disjoint; and
+// - their PRF table contents correctly refines their AEAD logs,
+//     (up to early decryptor allocations in initial state)
+
+// This invariant depends only on AEAD-writer regions and the PRF region. 
+//
+// During AE encrypt, the invariant is eventually restored as we extend the AEAD log, 
+// using a precise record of all entries added to the PRF table during encryption.
+//
+// During AE decrypt, the only interesting case is when early
+// verification fails: the invariant is restored for an extended PRF
+// state with an extra MAC in its initial state.
+//
+// For convenience, 'refines' relies on both the log and the table being ordered chronologically.
+
+// TODO `Functional' correctness? (actually a witnessed, stable property)
+// c = encryptT h i st nonce ad (real_or_zero i p) 
+//
+// Ideally, this depends on the (increasing) states of 
+// both the PRF and its MACs, and may follow from the global invariant.
+//
+// Really, this depends on the functional correctness of PRF. 
+// Needed: prf_read returning a ghost of the actual underlying block. 
+//let sub s start len = Seq.slice start (start+len) s // more convenient? 
